thys/JinjaThreads/Compiler/J1Heap.thy
@@ -14,7 +14,7 @@ locale J1_heap_base = heap_base +
   and thread_id2addr :: "'thread_id \<Rightarrow> 'addr"
   and sc_spurious_wakeups :: bool
   and empty_heap :: "'heap"
-  and allocate :: "'heap \<Rightarrow> htype \<Rightarrow> ('heap \<times> 'addr option)"
+  and allocate :: "'heap \<Rightarrow> htype \<Rightarrow> ('heap \<times> 'addr) set"
   and typeof_addr :: "'heap \<Rightarrow> 'addr \<rightharpoonup> htype"
   and heap_read :: "'heap \<Rightarrow> 'addr \<Rightarrow> addr_loc \<Rightarrow> 'addr val \<Rightarrow> bool"
   and heap_write :: "'heap \<Rightarrow> 'addr \<Rightarrow> addr_loc \<Rightarrow> 'addr val \<Rightarrow> 'heap \<Rightarrow> bool"
@@ -24,7 +24,7 @@ locale J1_heap = heap +
   and thread_id2addr :: "'thread_id \<Rightarrow> 'addr"
   and sc_spurious_wakeups :: bool
   and empty_heap :: "'heap"
-  and allocate :: "'heap \<Rightarrow> htype \<Rightarrow> ('heap \<times> 'addr option)"
+  and allocate :: "'heap \<Rightarrow> htype \<Rightarrow> ('heap \<times> 'addr) set"
   and typeof_addr :: "'heap \<Rightarrow> 'addr \<rightharpoonup> htype"
   and heap_read :: "'heap \<Rightarrow> 'addr \<Rightarrow> addr_loc \<Rightarrow> 'addr val \<Rightarrow> bool"
   and heap_write :: "'heap \<Rightarrow> 'addr \<Rightarrow> addr_loc \<Rightarrow> 'addr val \<Rightarrow> 'heap \<Rightarrow> bool"
@@ -37,7 +37,7 @@ locale J1_heap_conf_base = heap_conf_base +
   and thread_id2addr :: "'thread_id \<Rightarrow> 'addr"
   and sc_spurious_wakeups :: bool
   and empty_heap :: "'heap"
-  and allocate :: "'heap \<Rightarrow> htype \<Rightarrow> ('heap \<times> 'addr option)"
+  and allocate :: "'heap \<Rightarrow> htype \<Rightarrow> ('heap \<times> 'addr) set"
   and typeof_addr :: "'heap \<Rightarrow> 'addr \<rightharpoonup> htype"
   and heap_read :: "'heap \<Rightarrow> 'addr \<Rightarrow> addr_loc \<Rightarrow> 'addr val \<Rightarrow> bool"
   and heap_write :: "'heap \<Rightarrow> 'addr \<Rightarrow> addr_loc \<Rightarrow> 'addr val \<Rightarrow> 'heap \<Rightarrow> bool"
@@ -53,7 +53,7 @@ locale J1_heap_conf =
   and thread_id2addr :: "'thread_id \<Rightarrow> 'addr"
   and sc_spurious_wakeups :: bool
   and empty_heap :: "'heap"
-  and allocate :: "'heap \<Rightarrow> htype \<Rightarrow> ('heap \<times> 'addr option)"
+  and allocate :: "'heap \<Rightarrow> htype \<Rightarrow> ('heap \<times> 'addr) set"
   and typeof_addr :: "'heap \<Rightarrow> 'addr \<rightharpoonup> htype"
   and heap_read :: "'heap \<Rightarrow> 'addr \<Rightarrow> addr_loc \<Rightarrow> 'addr val \<Rightarrow> bool"
   and heap_write :: "'heap \<Rightarrow> 'addr \<Rightarrow> addr_loc \<Rightarrow> 'addr val \<Rightarrow> 'heap \<Rightarrow> bool"
@@ -69,7 +69,7 @@ locale J1_conf_read =
   and thread_id2addr :: "'thread_id \<Rightarrow> 'addr"
   and sc_spurious_wakeups :: bool
   and empty_heap :: "'heap"
-  and allocate :: "'heap \<Rightarrow> htype \<Rightarrow> ('heap \<times> 'addr option)"
+  and allocate :: "'heap \<Rightarrow> htype \<Rightarrow> ('heap \<times> 'addr) set"
   and typeof_addr :: "'heap \<Rightarrow> 'addr \<rightharpoonup> htype"
   and heap_read :: "'heap \<Rightarrow> 'addr \<Rightarrow> addr_loc \<Rightarrow> 'addr val \<Rightarrow> bool"
   and heap_write :: "'heap \<Rightarrow> 'addr \<Rightarrow> addr_loc \<Rightarrow> 'addr val \<Rightarrow> 'heap \<Rightarrow> bool"
