thys/JinjaThreads/JVM/JVMExecInstr.thy
@@ -54,19 +54,19 @@ exec_instr_Load:
 
 | exec_instr_New:
  "exec_instr (New C) P t h stk loc C\<^isub>0 M\<^isub>0 pc frs = 
-  {let (h', ao) = allocate h (Class_type C)
-   in case ao of None \<Rightarrow> (\<epsilon>, \<lfloor>addr_of_sys_xcpt OutOfMemory\<rfloor>, h', (stk, loc, C\<^isub>0, M\<^isub>0, pc) # frs)
-             | Some a \<Rightarrow> (\<lbrace>NewHeapElem a (Class_type C)\<rbrace>, None, h', (Addr a # stk, loc, C\<^isub>0, M\<^isub>0, pc + 1)#frs) }"
+  (let HA = allocate h (Class_type C)
+   in if HA = {} then {(\<epsilon>, \<lfloor>addr_of_sys_xcpt OutOfMemory\<rfloor>, h, (stk, loc, C\<^isub>0, M\<^isub>0, pc) # frs)}
+      else (\<lambda>(h', a). (\<lbrace>NewHeapElem a (Class_type C)\<rbrace>, None, h', (Addr a # stk, loc, C\<^isub>0, M\<^isub>0, pc + 1)#frs)) ` HA)"
 
 | exec_instr_NewArray:
   "exec_instr (NewArray T) P t h stk loc C0 M0 pc frs =
-  { let si = the_Intg (hd stk);
-        i = nat (sint si)
-    in (if si <s 0
-        then (\<epsilon>, \<lfloor>addr_of_sys_xcpt NegativeArraySize\<rfloor>, h, (stk, loc, C0, M0, pc) # frs)
-        else (let (h', ao) = allocate h (Array_type T i)
-              in case ao of None \<Rightarrow> (\<epsilon>, \<lfloor>addr_of_sys_xcpt OutOfMemory\<rfloor>, h', (stk, loc, C0, M0, pc) # frs)
-                        | Some a \<Rightarrow> (\<lbrace>NewHeapElem a (Array_type T i)\<rbrace>, None, h', (Addr a # tl stk, loc, C0, M0, pc + 1) # frs))) }"
+  (let si = the_Intg (hd stk);
+       i = nat (sint si)
+   in (if si <s 0
+       then {(\<epsilon>, \<lfloor>addr_of_sys_xcpt NegativeArraySize\<rfloor>, h, (stk, loc, C0, M0, pc) # frs)}
+        else let HA = allocate h (Array_type T i)
+             in if HA = {} then {(\<epsilon>, \<lfloor>addr_of_sys_xcpt OutOfMemory\<rfloor>, h, (stk, loc, C0, M0, pc) # frs)}
+                else (\<lambda>(h', a). (\<lbrace>NewHeapElem a (Array_type T i)\<rbrace>, None, h', (Addr a # tl stk, loc, C0, M0, pc + 1) # frs)) ` HA))"
 
 | exec_instr_ALoad:
   "exec_instr ALoad P t h stk loc C0 M0 pc frs =
