thys/JinjaThreads/MM/JMM_Framework.thy
@@ -393,7 +393,7 @@ locale heap_multithreaded_base =
   and thread_id2addr :: "'thread_id \<Rightarrow> 'addr"
   and spurious_wakeups :: bool
   and empty_heap :: "'heap"
-  and allocate :: "'heap \<Rightarrow> htype \<Rightarrow> ('heap \<times> 'addr option)"
+  and allocate :: "'heap \<Rightarrow> htype \<Rightarrow> ('heap \<times> 'addr) set"
   and typeof_addr :: "'heap \<Rightarrow> 'addr \<rightharpoonup> htype"
   and heap_read :: "'heap \<Rightarrow> 'addr \<Rightarrow> addr_loc \<Rightarrow> 'addr val \<Rightarrow> bool"
   and heap_write :: "'heap \<Rightarrow> 'addr \<Rightarrow> addr_loc \<Rightarrow> 'addr val \<Rightarrow> 'heap \<Rightarrow> bool" 
@@ -436,7 +436,7 @@ locale heap_multithreaded =
   and thread_id2addr :: "'thread_id \<Rightarrow> 'addr"
   and spurious_wakeups :: bool
   and empty_heap :: "'heap"
-  and allocate :: "'heap \<Rightarrow> htype \<Rightarrow> ('heap \<times> 'addr option)"
+  and allocate :: "'heap \<Rightarrow> htype \<Rightarrow> ('heap \<times> 'addr) set"
   and typeof_addr :: "'heap \<Rightarrow> 'addr \<rightharpoonup> htype"
   and heap_read :: "'heap \<Rightarrow> 'addr \<Rightarrow> addr_loc \<Rightarrow> 'addr val \<Rightarrow> bool"
   and heap_write :: "'heap \<Rightarrow> 'addr \<Rightarrow> addr_loc \<Rightarrow> 'addr val \<Rightarrow> 'heap \<Rightarrow> bool" 
@@ -725,7 +725,7 @@ locale allocated_multithreaded =
   and thread_id2addr :: "'thread_id \<Rightarrow> 'addr"
   and spurious_wakeups :: bool
   and empty_heap :: "'heap"
-  and allocate :: "'heap \<Rightarrow> htype \<Rightarrow> ('heap \<times> 'addr option)"
+  and allocate :: "'heap \<Rightarrow> htype \<Rightarrow> ('heap \<times> 'addr) set"
   and typeof_addr :: "'heap \<Rightarrow> 'addr \<rightharpoonup> htype"
   and heap_read :: "'heap \<Rightarrow> 'addr \<Rightarrow> addr_loc \<Rightarrow> 'addr val \<Rightarrow> bool"
   and heap_write :: "'heap \<Rightarrow> 'addr \<Rightarrow> addr_loc \<Rightarrow> 'addr val \<Rightarrow> 'heap \<Rightarrow> bool" 
@@ -1201,7 +1201,7 @@ locale known_addrs =
   and thread_id2addr :: "'thread_id \<Rightarrow> 'addr"
   and spurious_wakeups :: bool
   and empty_heap :: "'heap"
-  and allocate :: "'heap \<Rightarrow> htype \<Rightarrow> ('heap \<times> 'addr option)"
+  and allocate :: "'heap \<Rightarrow> htype \<Rightarrow> ('heap \<times> 'addr) set"
   and typeof_addr :: "'heap \<Rightarrow> 'addr \<rightharpoonup> htype"
   and heap_read :: "'heap \<Rightarrow> 'addr \<Rightarrow> addr_loc \<Rightarrow> 'addr val \<Rightarrow> bool"
   and heap_write :: "'heap \<Rightarrow> 'addr \<Rightarrow> addr_loc \<Rightarrow> 'addr val \<Rightarrow> 'heap \<Rightarrow> bool" 
@@ -1561,7 +1561,7 @@ locale known_addrs_typing =
   and thread_id2addr :: "'thread_id \<Rightarrow> 'addr"
   and spurious_wakeups :: bool
   and empty_heap :: "'heap"
-  and allocate :: "'heap \<Rightarrow> htype \<Rightarrow> ('heap \<times> 'addr option)"
+  and allocate :: "'heap \<Rightarrow> htype \<Rightarrow> ('heap \<times> 'addr) set"
   and typeof_addr :: "'heap \<Rightarrow> 'addr \<rightharpoonup> htype"
   and heap_read :: "'heap \<Rightarrow> 'addr \<Rightarrow> addr_loc \<Rightarrow> 'addr val \<Rightarrow> bool"
   and heap_write :: "'heap \<Rightarrow> 'addr \<Rightarrow> addr_loc \<Rightarrow> 'addr val \<Rightarrow> 'heap \<Rightarrow> bool" 
