thys/JinjaThreads/MM/JMM_JVM_Typesafe.thy
@@ -33,7 +33,7 @@ locale JVM_allocated_heap_conf' =
   and thread_id2addr :: "'thread_id \<Rightarrow> 'addr"
   and spurious_wakeups :: bool
   and empty_heap :: "'heap"
-  and allocate :: "'heap \<Rightarrow> htype \<Rightarrow> ('heap \<times> 'addr option)"
+  and allocate :: "'heap \<Rightarrow> htype \<Rightarrow> ('heap \<times> 'addr) set"
   and typeof_addr :: "'addr \<rightharpoonup> htype"
   and heap_read :: "'heap \<Rightarrow> 'addr \<Rightarrow> addr_loc \<Rightarrow> 'addr val \<Rightarrow> bool"
   and heap_write :: "'heap \<Rightarrow> 'addr \<Rightarrow> addr_loc \<Rightarrow> 'addr val \<Rightarrow> 'heap \<Rightarrow> bool"
@@ -141,7 +141,7 @@ lemma exec_instr_heap_read_typed:
 apply(cases i)
 apply(simp_all add: JVM_heap_base.exec_instr.simps split_beta cong: conj_cong)
 
-apply(auto dest: heap_base.heap_read_typed_into_heap_read)[2]
+apply(auto dest: heap_base.heap_read_typed_into_heap_read)[4]
 apply(blast dest:  heap_base.heap_read_typed_typed heap_base'.addr_loc_type_conv_addr_loc_type[THEN fun_cong, THEN fun_cong, THEN fun_cong, THEN iffD2] heap_base'.conf_conv_conf[THEN fun_cong, THEN fun_cong, THEN iffD1])
 apply(auto dest: heap_base'.addr_loc_type_conv_addr_loc_type[THEN fun_cong, THEN fun_cong, THEN fun_cong, THEN iffD1] intro: heap_base'.conf_conv_conf[THEN fun_cong, THEN fun_cong, THEN iffD2] heap_base.heap_read_typedI)[1]
 apply(blast dest:  heap_base.heap_read_typed_typed heap_base'.addr_loc_type_conv_addr_loc_type[THEN fun_cong, THEN fun_cong, THEN fun_cong, THEN iffD2] heap_base'.conf_conv_conf[THEN fun_cong, THEN fun_cong, THEN iffD1])
@@ -198,9 +198,9 @@ lemma jmm'_exec_instrI:
      final_thread.actions_ok (final_thread.init_fin_final JVM_final) s t ta \<rbrakk>
   \<Longrightarrow> \<exists>ta xcphfrs. (ta, xcphfrs) \<in> JVM_heap_base.exec_instr addr2thread_id thread_id2addr spurious_wakeups empty_heap allocate typeof_addr (heap_base.heap_read_typed typeof_addr jmm_heap_read P) jmm_heap_write i P t h stk loc C M pc frs \<and> final_thread.actions_ok (final_thread.init_fin_final JVM_final) s t ta"
 apply(cases i)
-apply(auto simp add: JVM_heap_base.exec_instr.simps split_beta final_thread.actions_ok_iff intro!: jmm_heap_read_typed_default_val simp del: split_paired_Ex split: split_if_asm)
+apply(auto simp add: JVM_heap_base.exec_instr.simps split_beta final_thread.actions_ok_iff intro!: jmm_heap_read_typed_default_val rev_image_eqI simp del: split_paired_Ex split: split_if_asm)
 apply(drule red_external_aggr_heap_read_typedI)
-apply(fastforce simp add: final_thread.actions_ok_iff simp del: split_paired_Ex)+
+apply((fastforce simp add: final_thread.actions_ok_iff simp del: split_paired_Ex)+)[2]
 done
 
 lemma jmm'_execI:
