thys/JinjaThreads/MM/JMM_J_Typesafe.thy
@@ -32,7 +32,7 @@ locale J_allocated_heap_conf' =
   and thread_id2addr :: "'thread_id \<Rightarrow> 'addr"
   and spurious_wakeups :: bool
   and empty_heap :: "'heap"
-  and allocate :: "'heap \<Rightarrow> htype \<Rightarrow> ('heap \<times> 'addr option)"
+  and allocate :: "'heap \<Rightarrow> htype \<Rightarrow> ('heap \<times> 'addr) set"
   and typeof_addr :: "'addr \<rightharpoonup> htype"
   and heap_read :: "'heap \<Rightarrow> 'addr \<Rightarrow> addr_loc \<Rightarrow> 'addr val \<Rightarrow> bool"
   and heap_write :: "'heap \<Rightarrow> 'addr \<Rightarrow> addr_loc \<Rightarrow> 'addr val \<Rightarrow> 'heap \<Rightarrow> bool"
